src/proofsearch/Search_Completeness.v
@@ -1,25 +1,26 @@
 From Stdlib Require Import List SetoidList.
-From LJF Require Import SharedLogic Predicates Sequents Pndctx Search_Procedure LJFPS_Rules LJFh_Rules Schemes Subsequent_Preservation.
+From LJF Require Import SharedLogic Predicates Sequents Pndctx Search_Procedure LJFPS_Rules LJFh_Rules Schemes Subsequent_Preservation ProofTerms.
 From Equations Require Import Equations.
 
-Definition returns_some_proof {A B : Prop} (r : option ({A} + {B})) : Prop :=
-  match r with Some (left _) => True | _ => False end.
+Definition returns_some_proof {A B : Type} (r : option (A + B)) : Prop :=
+  match r with Some (inl _) => True | _ => False end.
 
-Definition returns_some_disproof {A B : Prop} (r : option ({A} + {B})) : Prop :=
-  match r with Some (right _) => True | _ => False end.
+Definition returns_some_disproof {A B : Type} (r : option (A + B)) : Prop :=
+  match r with Some (inr _) => True | _ => False end.
 
-Definition returns_none {A B : Prop} (r : option ({A} + {B})) : Prop :=
+Definition returns_none {A B : Type} (r : option (A + B)) : Prop :=
   match r with None => True | _ => False end.
 
-Lemma returns_some_proof_inv {A B : Prop} {r : option ({A} + {B})} :
-  returns_some_proof r -> exists p : A, r = Some (left p).
+Lemma returns_some_proof_inv [A B: Type] {r : option (A + B)} :
+  returns_some_proof r -> exists p : A, r = Some (inl p).
 Proof.
     intros. destruct r as [[s | s]|] ; try contradiction.
     eexists s. reflexivity.
 Qed.
 
 Lemma try_Lf_complete :
-    forall (C : pndctx) (K : o) (try_N : forall N : o, In N (pndctx_list C) -> option (sumbool (lfc C N K) (~ lfc C N K)))
+    forall (C : pndctx) (K : o) 
+        (try_N : forall N : o, In N (pndctx_list C) -> option ({p : pterm | verify p (Slfc C N K)} + (~ sequent_derivable (Slfc C N K))))
             (neg_ctx : list o)
             (H_Forall : Forall (fun N : o => In N (pndctx_list C) /\ negative N) neg_ctx)
             (M : o), 
@@ -31,19 +32,19 @@ Proof.
     - inversion H.
     - destruct H ; subst.
         + specialize (H0 (proj1 (Forall_inv H_Forall))). simp try_Lf.
-            apply returns_some_proof_inv in H0. destruct H0. rewrite H. simpl. apply I.
+            apply returns_some_proof_inv in H0. destruct H0 as [[x v] H]. rewrite H. simpl. apply I.
         + specialize (IHneg_ctx (Forall_inv_tail H_Forall) M H H0).
             apply returns_some_proof_inv in IHneg_ctx. destruct IHneg_ctx. simp try_Lf.
             destruct (try_N a (proj1 (Forall_inv H_Forall))).
             destruct s.
-            -- simpl. apply I.
-            -- simpl. rewrite H1. simpl. apply I.
-            -- simpl. rewrite H1. simpl. apply I.
+            -- destruct s. simpl. apply I.
+            -- destruct x. simpl. rewrite H1. simpl. apply I.
+            -- destruct x. simpl. rewrite H1. simpl. apply I.
 Qed.
                 
 Lemma try_Lf_wrapper_complete :
     forall (C : pndctx) (K : o) 
-            (try_N : forall N : o, In N (pndctx_list C) -> option (sumbool (lfc C N K) (~ lfc C N K)))
+            (try_N : forall N : o, In N (pndctx_list C) ->  option ({p : pterm | verify p (Slfc C N K)} + (~ sequent_derivable (Slfc C N K))))
             (M : o),
         In M (pndctx_list C) ->
         negative M ->
@@ -93,33 +94,33 @@ Proof.
     - destruct D ; simp search ; cbv zeta.
         + destruct p ; simp search ; cbv zeta.
             -- specialize (H init (subp_bct_boxR (Bracketable_pos (Atom Pos n) (Pos_atom n)) Hsub) Hstack_NoDup Hstack_sub).
-                apply returns_some_proof_inv in H. destruct H.
+                apply returns_some_proof_inv in H. destruct H as [[x v] H].
                 rewrite H. simpl. apply I.
             -- specialize (H init (subp_bct_boxR (Bracketable_neg_atom (Atom Neg n) (Is_atom Neg n) (Neg_atom n)) Hsub) Hstack_NoDup Hstack_sub).
-                apply returns_some_proof_inv in H. destruct H.
+                apply returns_some_proof_inv in H. destruct H as [[x v] H].
                 rewrite H. simpl. apply I.
         + specialize (H init (subp_bct_boxR (Bracketable_pos TT Pos_true) Hsub) Hstack_NoDup Hstack_sub).
-            apply returns_some_proof_inv in H. destruct H.
+            apply returns_some_proof_inv in H. destruct H as [[x v] H].
                 rewrite H. simpl. apply I.
         + specialize (H init (subp_bct_boxR (Bracketable_pos FF Pos_false) Hsub) Hstack_NoDup Hstack_sub).
-            apply returns_some_proof_inv in H. destruct H.
+            apply returns_some_proof_inv in H. destruct H as [[x v] H].
             rewrite H. simpl. apply I.
         + specialize (H init (subp_bct_boxR (Bracketable_pos (AndP D1 D2) (Pos_and D1 D2)) Hsub) Hstack_NoDup Hstack_sub).
-            apply returns_some_proof_inv in H. destruct H.
+            apply returns_some_proof_inv in H. destruct H as [[x v] H].
             rewrite H. simpl. apply I.
         + inversion b ; inversion H0.
         + specialize (H init (subp_bct_boxR (Bracketable_pos (Or D1 D2) (Pos_or D1 D2)) Hsub) Hstack_NoDup Hstack_sub).
-            apply returns_some_proof_inv in H. destruct H.
+            apply returns_some_proof_inv in H. destruct H as [[x v] H].
             rewrite H. simpl. apply I.
         + inversion b ; inversion H0.
     - simp search.
         specialize (H init (proj1 (subp_bct_AndNR Hsub)) Hstack_NoDup Hstack_sub).
-        apply returns_some_proof_inv in H. destruct H. rewrite H. simpl. 
+        apply returns_some_proof_inv in H. destruct H as [[x v] H]. rewrite H. simpl. 
         specialize (H0 init (proj2 (subp_bct_AndNR Hsub)) Hstack_NoDup Hstack_sub).
-        apply returns_some_proof_inv in H0. destruct H0. cbn in H0. cbn. rewrite H0. simpl. apply I.
+        apply returns_some_proof_inv in H0. destruct H0 as [[x0 v0] H0]. cbn in H0. cbn. rewrite H0. simpl. apply I.
     - simp search.
         specialize (H init (subp_bct_ImpR Hsub) Hstack_NoDup Hstack_sub).
-        apply returns_some_proof_inv in H. destruct H.
+        apply returns_some_proof_inv in H. destruct H as [[x v] H].
         rewrite H. simpl. apply I.
     - rewrite search_equation_9. destruct (InA_dec (eqA:=pndctx_o_eq) pndctx_o_eq_dec (C, K) Hs).
         + contradiction.
@@ -130,58 +131,58 @@ Proof.
                         search init (Slfc C N0 K) (subp_ept_Lf HinN Hsub) ((C, K) :: Hs) (NoDupA_cons n1 Hstack_NoDup)  (Forall_cons (C, K) Hsub Hstack_sub)))).
             -- apply (try_Lf_wrapper_complete C K _ N i n0). intros.
                 specialize (H init (subp_ept_Lf Hin Hsub) (NoDupA_cons n1 Hstack_NoDup) (Forall_cons (C, K) Hsub Hstack_sub)).
-                apply returns_some_proof_inv in H. destruct H. rewrite H. simpl. apply I.
+                apply returns_some_proof_inv in H. destruct H as [[x v] H]. rewrite H. simpl. apply I.
             -- destruct (Decidability.positive_dec K).
                 ++ simp search. destruct (search init (Srfc C K) (subp_ept_Rf Hsub) ((C, K) :: Hs) (NoDupA_cons (x:=(C, K)) n1 Hstack_NoDup) (Forall_cons (C, K) Hsub Hstack_sub)).
                     --- destruct s.
-                        +++ simpl. apply I.
-                        +++ simpl. apply returns_some_proof_inv in H0. destruct H0. cbn in H0. cbn. rewrite H0. simpl. apply I.
-                    --- simpl. apply returns_some_proof_inv in H0. destruct H0. cbn in H0. cbn. rewrite H0. simpl. apply I.
-                ++ simp search. apply returns_some_proof_inv in H0. destruct H0. cbn in H0. cbn. rewrite H0. simpl. apply I.
+                        +++ destruct s. simpl. apply I.
+                        +++ simpl. apply returns_some_proof_inv in H0. destruct H0 as [[x0 v0] H0]. cbn in H0. cbn. rewrite H0. simpl. apply I.
+                    --- simpl. apply returns_some_proof_inv in H0. destruct H0 as [[x0 v0] H0]. cbn in H0. cbn. rewrite H0. simpl. apply I.
+                ++ simp search. apply returns_some_proof_inv in H0. destruct H0 as [[x0 v0] H0]. cbn in H0. cbn. rewrite H0. simpl. apply I.
     - rewrite search_equation_9. destruct (InA_dec (eqA:=pndctx_o_eq) pndctx_o_eq_dec (C, P) Hs).
         + contradiction.
         + simpl. destruct (Decidability.positive_dec P).
             -- simpl. specialize (H init (subp_ept_Rf Hsub) (NoDupA_cons (x:=(C, P)) n0 Hstack_NoDup) (Forall_cons (C, P) Hsub Hstack_sub)).
-                apply returns_some_proof_inv in H. destruct H. cbn in H. cbn. rewrite H. simpl. apply I.
+                apply returns_some_proof_inv in H. destruct H as [[x v] H]. cbn in H. cbn. rewrite H. simpl. apply I.
             -- contradiction.
     - destruct B ; simp search ; cbv zeta ; try (solve [inversion p ; inversion H0]).
         + destruct p0 ; simp search ; cbv zeta.
             -- specialize (H init (subp_ept_boxL Hsub) Hstack_NoDup Hstack_sub).
-                apply returns_some_proof_inv in H. destruct H.
+                apply returns_some_proof_inv in H. destruct H as [[x v] H].
                 rewrite H. simpl. apply I.
             -- specialize (H init (subp_ept_boxL Hsub) Hstack_NoDup Hstack_sub).
-                apply returns_some_proof_inv in H. destruct H.
+                apply returns_some_proof_inv in H. destruct H as [[x v] H].
                 rewrite H. simpl. apply I.
         + specialize (H init (subp_ept_boxL Hsub) Hstack_NoDup Hstack_sub).
-            apply returns_some_proof_inv in H. destruct H. rewrite H. simpl. apply I.
+            apply returns_some_proof_inv in H. destruct H as [[x v] H]. rewrite H. simpl. apply I.
         + specialize (H init (subp_ept_boxL Hsub) Hstack_NoDup Hstack_sub).
-            apply returns_some_proof_inv in H. destruct H. rewrite H. simpl. apply I.
+            apply returns_some_proof_inv in H. destruct H as [[x v] H]. rewrite H. simpl. apply I.
     - simp search.
         specialize (H init (subp_ept_AndPL Hsub) Hstack_NoDup Hstack_sub).
-        apply returns_some_proof_inv in H. destruct H. rewrite H. simpl. apply I.
+        apply returns_some_proof_inv in H. destruct H as [[x v] H]. rewrite H. simpl. apply I.
     - simp search.
         specialize (H init (proj1 (subp_ept_OrL Hsub)) Hstack_NoDup Hstack_sub).
-        apply returns_some_proof_inv in H. destruct H. rewrite H. simpl.
+        apply returns_some_proof_inv in H. destruct H as [[x v] H]. rewrite H. simpl.
         specialize (H0 init (proj2 (subp_ept_OrL Hsub)) Hstack_NoDup Hstack_sub).
-        apply returns_some_proof_inv in H0. destruct H0. cbn in H0. cbn. rewrite H0. simpl. apply I.
+        apply returns_some_proof_inv in H0. destruct H0 as [[x0 v0] H0]. cbn in H0. cbn. rewrite H0. simpl. apply I.
     - simp search.
         specialize (H init (subp_ept_TrueL Hsub) Hstack_NoDup Hstack_sub).
-        apply returns_some_proof_inv in H. destruct H. rewrite H. simpl. apply I.
+        apply returns_some_proof_inv in H. destruct H as [[x v] H]. rewrite H. simpl. apply I.
     - simp search.
         destruct (Decidability.bracketable_dec K).
         + simpl. apply I.
         + contradiction.
     - inversion p ; subst.
         + rewrite search_equation_18 ; cbv zeta.
-            specialize (H init (subp_lfc_Rl Hsub) Hstack_NoDup Hstack_sub). apply returns_some_proof_inv in H. destruct H. rewrite H. simpl. apply I.
+            specialize (H init (subp_lfc_Rl Hsub) Hstack_NoDup Hstack_sub). apply returns_some_proof_inv in H. destruct H as [[x v] H]. rewrite H. simpl. apply I.
         + rewrite search_equation_20 ; cbv zeta.
-            specialize (H init (subp_lfc_Rl Hsub) Hstack_NoDup Hstack_sub). apply returns_some_proof_inv in H. destruct H. rewrite H. simpl. apply I.
+            specialize (H init (subp_lfc_Rl Hsub) Hstack_NoDup Hstack_sub). apply returns_some_proof_inv in H. destruct H as [[x v] H]. rewrite H. simpl. apply I.
         + rewrite search_equation_21 ; cbv zeta.
-            specialize (H init (subp_lfc_Rl Hsub) Hstack_NoDup Hstack_sub). apply returns_some_proof_inv in H. destruct H. rewrite H. simpl. apply I.
+            specialize (H init (subp_lfc_Rl Hsub) Hstack_NoDup Hstack_sub). apply returns_some_proof_inv in H. destruct H as [[x v] H]. rewrite H. simpl. apply I.
         + rewrite search_equation_22 ; cbv zeta.
-            specialize (H init (subp_lfc_Rl Hsub) Hstack_NoDup Hstack_sub). apply returns_some_proof_inv in H. destruct H. rewrite H. simpl. apply I.
+            specialize (H init (subp_lfc_Rl Hsub) Hstack_NoDup Hstack_sub). apply returns_some_proof_inv in H. destruct H as [[x v] H]. rewrite H. simpl. apply I.
         + rewrite search_equation_24 ; cbv zeta.
-            specialize (H init (subp_lfc_Rl Hsub) Hstack_NoDup Hstack_sub). apply returns_some_proof_inv in H. destruct H. rewrite H. simpl. apply I.
+            specialize (H init (subp_lfc_Rl Hsub) Hstack_NoDup Hstack_sub). apply returns_some_proof_inv in H. destruct H as [[x v] H]. rewrite H. simpl. apply I.
     - inversion n.
         + inversion a ; subst.
             simp search.
@@ -192,44 +193,44 @@ Proof.
         + inversion a ; subst. inversion H0.
     - simp search.
         specialize (H init (subp_lfc_AndNL_1 Hsub) Hstack_NoDup Hstack_sub).
-        apply returns_some_proof_inv in H. destruct H. rewrite H. simpl. apply I.
+        apply returns_some_proof_inv in H. destruct H as [[x v] H]. rewrite H. simpl. apply I.
     - rewrite search_equation_23.
-        specialize (H init (subp_lfc_AndNL_2 Hsub) Hstack_NoDup Hstack_sub). apply returns_some_proof_inv in H. destruct H.
+        specialize (H init (subp_lfc_AndNL_2 Hsub) Hstack_NoDup Hstack_sub). apply returns_some_proof_inv in H. destruct H as [[x v] H].
         destruct (search init (Slfc C B1 K) (subp_lfc_AndNL_1 Hsub) Hs Hstack_NoDup Hstack_sub).
         + destruct s.
-            -- simpl. apply I.
+            -- destruct s. simpl. apply I.
             -- simpl. rewrite H. simpl. apply I.
         + simpl. rewrite H. simpl. apply I.
     - simp search.
         specialize (H init (proj1 (subp_lfc_ImpL Hsub)) Hstack_NoDup Hstack_sub).
-        apply returns_some_proof_inv in H. destruct H. rewrite H. simpl.
+        apply returns_some_proof_inv in H. destruct H as [[x v] H]. rewrite H. simpl.
         specialize (H0 init (proj2 (subp_lfc_ImpL Hsub)) Hstack_NoDup Hstack_sub).
-        apply returns_some_proof_inv in H0. destruct H0. cbn in H0. cbn. rewrite H0. simpl. apply I.
+        apply returns_some_proof_inv in H0. destruct H0 as [[x0 v0] H0]. cbn in H0. cbn. rewrite H0. simpl. apply I.
     - inversion n ; subst.
         + rewrite search_equation_27 ; cbv zeta.
-            specialize (H init (subp_rfc_Rr Hsub) Hstack_NoDup Hstack_sub). apply returns_some_proof_inv in H. destruct H. rewrite H. simpl. apply I.
+            specialize (H init (subp_rfc_Rr Hsub) Hstack_NoDup Hstack_sub). apply returns_some_proof_inv in H. destruct H as [[x v] H]. rewrite H. simpl. apply I.
         + rewrite search_equation_31 ; cbv zeta.
-            specialize (H init (subp_rfc_Rr Hsub) Hstack_NoDup Hstack_sub). apply returns_some_proof_inv in H. destruct H. rewrite H. simpl. apply I.
+            specialize (H init (subp_rfc_Rr Hsub) Hstack_NoDup Hstack_sub). apply returns_some_proof_inv in H. destruct H as [[x v] H]. rewrite H. simpl. apply I.
         + rewrite search_equation_33 ; cbv zeta.
-            specialize (H init (subp_rfc_Rr Hsub) Hstack_NoDup Hstack_sub). apply returns_some_proof_inv in H. destruct H. rewrite H. simpl. apply I.
+            specialize (H init (subp_rfc_Rr Hsub) Hstack_NoDup Hstack_sub). apply returns_some_proof_inv in H. destruct H as [[x v] H]. rewrite H. simpl. apply I.
     - inversion p ; inversion a ; subst ; inversion H0. subst. simp search. 
         destruct (in_dec Decidability.o_eq_dec (Atom Pos n) (pndctx_list C)).
         + simpl. apply I.
         + contradiction.
     - simp search.
         specialize (H init (proj1 (subp_rfc_AndPR Hsub)) Hstack_NoDup Hstack_sub).
-        apply returns_some_proof_inv in H. destruct H. rewrite H. simpl.
+        apply returns_some_proof_inv in H. destruct H as [[x v] H]. rewrite H. simpl.
         specialize (H0 init (proj2 (subp_rfc_AndPR Hsub)) Hstack_NoDup Hstack_sub).
-        apply returns_some_proof_inv in H0. destruct H0. cbn in H0. cbn. rewrite H0. simpl. apply I.
+        apply returns_some_proof_inv in H0. destruct H0 as [[x0 v0] H0]. cbn in H0. cbn. rewrite H0. simpl. apply I.
     - simp search.
         specialize (H init (subp_rfc_OrR_1 Hsub) Hstack_NoDup Hstack_sub).
-        apply returns_some_proof_inv in H. destruct H. rewrite H. simpl. apply I.
+        apply returns_some_proof_inv in H. destruct H as [[x v] H]. rewrite H. simpl. apply I.
     - rewrite search_equation_32.
         specialize (H init (subp_rfc_OrR_2 Hsub) Hstack_NoDup Hstack_sub).
-        apply returns_some_proof_inv in H ; destruct H.
+        apply returns_some_proof_inv in H ; destruct H as [[x v] H].
         destruct (search init (Srfc C B1) (subp_rfc_OrR_1 Hsub) Hs Hstack_NoDup Hstack_sub).
         + destruct s.
-            -- simpl. apply I.
+            -- destruct s. simpl. apply I.
             -- simpl. rewrite H. simpl. apply I.
         + simpl. rewrite H. simpl. apply I.
     - simp search. simpl. apply I.
